ulib/FStar.BufferNG.fst
@@ -810,7 +810,7 @@ let locset_dead_locset_of_buffer_liveness_tag
   (h: HS.mem)
   (b: buffer t)
 : Lemma
-  (ensures (Modifies.locset_dead (locset_of_buffer_liveness_tag b) h <==> (~ (contains h b))))
+  (ensures (Modifies.locset_dead h (locset_of_buffer_liveness_tag b) <==> (~ (contains h b))))
 = Classical.forall_intro_3 (fun t -> Pointer.locset_dead_locset_of_pointer_liveness_tag #t)
 
 abstract
@@ -819,7 +819,7 @@ let locset_dead_locset_of_buffer
   (h: HS.mem)
   (b: buffer t)
 : Lemma
-  (ensures (Modifies.locset_dead (locset_of_buffer b) h <==> (~ (contains h b))))
+  (ensures (Modifies.locset_dead h (locset_of_buffer b) <==> (~ (contains h b))))
 = Modifies.loc_of_object_inj_forall HS.root_class;
   Classical.forall_intro_3 (fun t -> Pointer.locset_dead_locset_of_pointer_liveness_tag #t);
   Classical.forall_intro_3 (fun t -> Pointer.locset_dead_locset_of_pointer #t)
@@ -831,7 +831,7 @@ let locset_dead_locset_of_buffer_contents
   (b: buffer t)
 : Lemma
   (requires (~ (contains h b)))
-  (ensures (Modifies.locset_dead (locset_of_buffer_contents b) h))
+  (ensures (Modifies.locset_dead h (locset_of_buffer_contents b)))
 = Modifies.loc_of_object_inj_forall HS.root_class;
   Classical.forall_intro_3 (fun t -> Pointer.locset_dead_locset_of_pointer #t)
 
@@ -844,7 +844,7 @@ val create: #a:Type -> init:a -> len:UInt32.t -> StackInline (buffer a)
      /\ live h1 b /\ length b = len
 //     /\ frameOf b = h0.tip // TODO: support frameOf
      /\ Modifies.modifies u#0 u#1 (TSet.empty #(Modifies.loc HS.root_class)) h0 h1
-     /\ Modifies.locset_dead (locset_of_buffer b) h0
+     /\ Modifies.locset_dead h0 (locset_of_buffer b)
      /\ as_seq h1 b == Seq.create (UInt32.v len) init))
 let create #a init len =
   let h0 = HST.get () in
@@ -852,7 +852,7 @@ let create #a init len =
     Pointer.screate' (Seq.create (UInt32.v len) init)
   in
   let b = buffer_of_array_pointer content in  
-  let _ : squash (Modifies.locset_dead (locset_of_buffer b) h0) =
+  let _ : squash (Modifies.locset_dead h0 (locset_of_buffer b)) =
     Modifies.loc_of_object_inj_forall HS.root_class;
     Classical.forall_intro_3 (fun t -> Pointer.locset_dead_locset_of_pointer_with_liveness #t)
   in
@@ -864,7 +864,7 @@ val rcreate: #a:Type -> r:HH.rid -> init:a -> len:UInt32.t -> ST (buffer a)
   (ensures (fun (h0: HS.mem) b h1 -> ~(contains h0 b)
     /\ live h1 b /\ length b = len
     /\ Modifies.modifies u#0 u#1 (TSet.empty #(Modifies.loc HS.root_class)) h0 h1
-    /\ Modifies.locset_dead (locset_of_buffer b) h0
+    /\ Modifies.locset_dead h0 (locset_of_buffer b)
     /\ as_seq h1 b == Seq.create (UInt32.v len) init
 //    /\ ~(b.Heap.content.HS.mm) // TODO: support mm
   ))
@@ -875,7 +875,7 @@ let rcreate #a r init len =
     Pointer.ecreate' r s
   in
   let b = buffer_of_array_pointer content in
-  let _ : squash (Modifies.locset_dead (locset_of_buffer b) h0) =
+  let _ : squash (Modifies.locset_dead h0 (locset_of_buffer b)) =
     Modifies.loc_of_object_inj_forall HS.root_class;
     Classical.forall_intro_3 (fun t -> Pointer.locset_dead_locset_of_pointer_with_liveness #t)
   in
